Lifted the correctness result to the reflexive transitive closure of the compatible closure of the hoisting rewrite relation. Also proved the corollary that states that the hoisting function is correct.

theories/L6_PCPS/identifiers.v
@@ -1,5 +1,5 @@
 Require Import List BinNat Relations Coq.MSets.MSetRBT List Ensembles.
-Require Import cps cps_util set_util Ensembles_util.
+Require Import cps cps_util ctx set_util Ensembles_util.
 Import ListNotations.
 
 Import PS.
@@ -34,7 +34,7 @@ Proof.
   - right. intros Hc; inv Hc.
 Qed.
 
-(** [fun+in_fundefs B] is the set of functions defined in [B] *)
+(** [fun_in_fundefs B] is the set of functions defined in [B] *)
 Fixpoint fun_in_fundefs  (B : fundefs) : Ensemble (var * type * list var * exp) :=
   match B with
     | Fnil => Empty_set _
@@ -135,6 +135,93 @@ Proof.
   intros Hname Hfree. 
   induction Hfree; inversion Hname; eauto.
   inv H3. eauto. inv H0; eauto.
+Qed.
+
+Lemma occurs_free_Econstr x tau t ys e :
+  Same_set var (occurs_free (Econstr x tau t ys e))
+           (Union _ (FromList ys) (Setminus var (occurs_free e) (Singleton var x))).
+Proof.
+  split; intros x' H; inv H; eauto.
+  right. constructor; eauto. intros H. inv H; eauto.
+  inv H0. constructor 2; eauto. intros Hc. subst. eauto.
+Qed.
+
+Lemma occurs_free_Eprim x tau f ys e :
+  Same_set var (occurs_free (Eprim x tau f ys e))
+           (Union _ (FromList ys) (Setminus var (occurs_free e) (Singleton var x))).
+Proof.
+  split; intros x' H; inv H; eauto.
+  right. constructor; eauto. intros H. inv H; eauto.
+  inv H0. eapply Free_Eprim2; eauto. intros Hc. subst. eauto.
+Qed.
+
+Lemma occurs_free_Eproj x tau t y e :
+  Same_set var (occurs_free (Eproj x tau t y e))
+           (Union _ (Singleton var y) (Setminus var (occurs_free e) (Singleton var x))).
+Proof.
+  split; intros x' H; inv H; eauto. 
+  right. constructor; eauto. intros H. inv H; eauto.
+  inv H0. eauto.
+  inv H0. constructor; eauto.
+  intros Hc. subst. eauto.
+Qed.
+
+Lemma occurs_free_Eapp f ys :
+  Same_set var (occurs_free (Eapp f ys))
+           (Union _ (FromList ys) (Singleton var f)).
+Proof.
+  split; intros x' H; inv H; eauto. inv H0; eauto.
+Qed.
+
+Lemma occurs_free_Efun B e :
+  Same_set var (occurs_free (Efun B e))
+           (Union _ (occurs_free_fundefs B)
+                  (Setminus _ (occurs_free e) (name_in_fundefs B))).
+Proof.
+  split; intros x' H; inv H; eauto.
+  right; eauto. constructor; eauto.
+  inv H0. eauto. 
+Qed.
+
+Lemma occurs_free_Ecase_nil x :
+  Same_set var (occurs_free (Ecase x []))
+           (Singleton _ x).
+Proof.
+  split; intros x' H; inv H; eauto.
+Qed.
+
+Lemma occurs_free_Ecase_cons x c e P :
+  Same_set var (occurs_free (Ecase x ((c, e) :: P)))
+           (Union _ (occurs_free e)
+                  (Union _ (Singleton _ x)
+                         (occurs_free (Ecase x P)))).
+Proof.
+  split; intros x' H; inv H; eauto.
+  inv H0; eauto. inv H; eauto.
+Qed.
+  
+Lemma occurs_free_Ecase_app x c e P P' :
+  Same_set var (occurs_free (Ecase x (P' ++ ((c, e) :: P))))
+           (Union _ (occurs_free e)
+                  (Union _ (Singleton _ x)
+                         (Union _ (occurs_free (Ecase x P'))
+                                (occurs_free (Ecase x P))))).
+Proof.
+  induction P' as [| [c' e'] P' IHP']; simpl.
+  - rewrite occurs_free_Ecase_nil.
+    rewrite (Union_assoc (Singleton var x)), Union_idempotent.
+    now apply occurs_free_Ecase_cons.
+  - rewrite !occurs_free_Ecase_cons. rewrite IHP'.
+    rewrite  !Union_assoc. rewrite (Union_sym _ (occurs_free e)).
+    rewrite <- Union_assoc. rewrite (Union_sym (occurs_free e')).
+    rewrite  !Union_assoc. apply Same_set_refl.
+Qed.
+
+Lemma occurs_free_fundefs_Fcons_Included f tau xs e B :
+  Included var (occurs_free_fundefs B)
+           (Union _ (occurs_free_fundefs (Fcons f tau xs e B)) (Singleton var f)).
+Proof.
+  intros x H. destruct (var_dec f x); subst; now eauto.
 Qed.
 
 Lemma occurs_free_Econstr_Included x tau t ys e :
@@ -281,13 +368,18 @@ Inductive funs_in_exp : fundefs -> exp -> Prop :=
     forall fs e x tau t ys,
       funs_in_exp fs e ->
       funs_in_exp fs (Econstr x tau t ys e)
+| In_Case :
+    forall fs x c e P,
+      funs_in_exp fs e ->
+      List.In (c, e) P ->
+      funs_in_exp fs (Ecase x P)
 | In_Eproj :    
     forall fs e x tau N ys,
       funs_in_exp fs e ->
       funs_in_exp fs (Eproj x tau N ys e)
 | In_Fun1 :
     forall fs e,
-      funs_in_exp fs (Efun fs e)
+      funs_in_exp fs (Efun fs e)          
 | In_Fun2 :
     forall fs fs' e,
       funs_in_exp fs e ->
@@ -310,10 +402,19 @@ with funs_in_fundef : fundefs -> fundefs -> Prop :=
       funs_in_fundef fs fs' ->
       funs_in_fundef fs (Fcons x tau ys e fs').
 
+Hint Constructors funs_in_exp.
+Hint Constructors funs_in_fundef.
+
+
 (** all functions defined in an expression are closed *)
 Definition closed_fundefs_in_exp (e : exp) :=
   forall defs, funs_in_exp defs e -> closed_fundefs defs.
-  
+
+(** all nested functions defined in a function block are closed *)
+Definition closed_fundefs_in_fundefs (B : fundefs) := 
+  forall B' : fundefs, funs_in_fundef B' B -> closed_fundefs B'.
+
+
 (** bound variables - alternative definition without lists or 
     number of occurences *)
 Inductive bound_var : exp -> Ensemble var :=
@@ -365,6 +466,65 @@ with bound_var_fundefs : fundefs -> Ensemble var :=
       bound_var e x ->
       bound_var_fundefs (Fcons f tau ys e defs) x.
 
+Hint Constructors bound_var.
+Hint Constructors bound_var_fundefs.
+
+Lemma bound_var_Econstr x tau t ys e :
+  Same_set _ (bound_var (Econstr x tau t ys e))
+           (Union var (bound_var e) (Singleton _ x)).
+Proof.
+  split; intros x' H; inv H; eauto. inv H0; eauto.
+Qed.
+
+Lemma bound_var_Eproj x tau t y e :
+  Same_set _ (bound_var (Eproj x tau t y e))
+           (Union var (bound_var e) (Singleton _ x)).
+Proof.
+  split; intros x' H; inv H; eauto. inv H0; eauto.
+Qed.
+
+Lemma bound_var_Eprim x tau f y e :
+  Same_set _ (bound_var (Eprim x tau f y e))
+           (Union var (bound_var e) (Singleton _ x)).
+Proof.
+  split; intros x' H; inv H; eauto. inv H0; eauto.
+Qed.
+
+Lemma bound_var_Eapp f ys :
+  Same_set _ (bound_var (Eapp f ys))
+           (Empty_set var).
+Proof.
+  split; intros x' H; inv H; eauto.
+Qed.
+
+Lemma bound_var_Ecase_nil x  :
+  Same_set _ (bound_var (Ecase x []))
+           (Empty_set var).
+Proof.
+  split; intros x' H; inv H; eauto. inv H4.
+Qed.
+
+Lemma bound_var_Ecase_cons x c e P :
+  Same_set _ (bound_var (Ecase x ((c, e) :: P)))
+           (Union var (bound_var e) (bound_var (Ecase x P))).
+Proof.
+  split; intros x' H; inv H; eauto.
+  - inv H4; eauto. inv H; eauto.
+  - econstructor; eauto. left. eauto.
+  - inv H0. econstructor; eauto. right. eauto.
+Qed.
+
+Lemma bound_var_Ecase_append x P1 P2 :
+  Same_set _ (bound_var (Ecase x (P1 ++ P2)))
+           (Union var (bound_var (Ecase x P1)) (bound_var (Ecase x P2))).
+Proof.
+  induction P1 as [ | [c e] P1 IHP1]; simpl; eauto.
+  - rewrite bound_var_Ecase_nil, Union_Empty_set_r.
+    eapply Same_set_refl.
+  - simpl. rewrite !bound_var_Ecase_cons, IHP1, Union_assoc.
+    eapply Same_set_refl.
+Qed.
+
 (** unique bindings - alternative definition without lists *)
 Inductive unique_bindings : exp -> Prop :=
 | UBound_Econstr :
@@ -377,6 +537,15 @@ Inductive unique_bindings : exp -> Prop :=
       ~ (bound_var e) x ->
       unique_bindings e ->
       unique_bindings (Eproj x tau n y e)
+| UBound_Ecase1 :
+    forall x,
+      unique_bindings (Ecase x [])
+| UBound_Ecase2 :
+    forall x c e P,
+      unique_bindings (Ecase x P) ->
+      unique_bindings e ->
+      Disjoint var (bound_var e) (bound_var (Ecase x P)) ->
+      unique_bindings (Ecase x ((c, e) :: P))
 | UBound_Efun :
     forall defs e,
       unique_bindings e ->
@@ -488,19 +657,19 @@ Lemma occurs_free_fundefs_big_cup B :
   Same_set _ (occurs_free_fundefs B)
            (big_cup (fun_in_fundefs B)
                     (fun p =>
-                       let '(f, _, xs, e) := p in
-                       (Setminus _ (occurs_free e)
-                                 (Union _ (FromList xs) (name_in_fundefs B))))).
+                       (Setminus _ (let '(f, _, xs, e) := p in
+                                    (Setminus _ (occurs_free e) (FromList xs)))
+                                 (name_in_fundefs B)))).
 Proof.
   induction B; simpl.
   - rewrite occurs_free_fundefs_Fcons. rewrite IHB.
     rewrite Union_big_cup, big_cup_Singleton.
-    apply Same_set_Union_compat.
+    rewrite Setminus_Union. apply Same_set_Union_compat.
     rewrite (Union_assoc (FromList l)), (Union_sym _ (Singleton var v)),
             <- Union_assoc. apply Same_set_refl.
     rewrite <- Setminus_big_cup.
     apply Same_Set_big_cup_r. intros [[[f tau] xs] e'].
-    rewrite Setminus_Union, <- Union_assoc, (Union_sym (Singleton var v)).
+    rewrite Setminus_Union, (Union_sym (Singleton var v)).
     apply Same_set_refl.
   - rewrite occurs_free_fundefs_Fnil, big_cup_Empty_set. apply Same_set_refl.
 Qed.
@@ -524,8 +693,8 @@ Proof.
   rewrite !occurs_free_fundefs_big_cup. intros H.
   apply Same_Set_big_cup; eauto.
   intros [[[f tau] xs] e']. apply Same_set_Setminus_compat.
-  apply Same_set_refl. apply Same_set_Union_compat.
-  apply Same_set_refl. rewrite !name_in_fundefs_big_cup_fun_in_fundefs.
+  now apply Same_set_refl.
+  rewrite !name_in_fundefs_big_cup_fun_in_fundefs.
   apply Same_Set_big_cup_l; eauto.
 Qed.
   
@@ -537,10 +706,9 @@ Proof.
   intros Hspl1 Hspl2. rewrite !occurs_free_fundefs_big_cup.
   apply Same_Set_big_cup.
   - intros [[[f tau] xs] e']. apply Same_set_Setminus_compat.
-    apply Same_set_refl. apply Same_set_Union_compat.
-    apply Same_set_refl. rewrite !name_in_fundefs_big_cup_fun_in_fundefs.
+    now apply Same_set_refl. rewrite !name_in_fundefs_big_cup_fun_in_fundefs.
     apply Same_Set_big_cup_l; eauto. rewrite split_fds_fun_in_fundefs; eauto.
-    rewrite (split_fds_fun_in_fundefs B1 B2 B3'); eauto. apply Same_set_refl.
+    rewrite (split_fds_fun_in_fundefs B1 B2 B3'); eauto. now apply Same_set_refl.
   - rewrite split_fds_fun_in_fundefs; eauto.
     rewrite (split_fds_fun_in_fundefs B1 B2 B3'); eauto. apply Same_set_refl.
 Qed.
@@ -553,7 +721,68 @@ Proof.
   intros Hspl1 Hspl2 Hcl. unfold closed_fundefs in *.
   rewrite same_split_fds_closed_occurs_free_fundefs; eauto.
 Qed.
-  
+
+Lemma unique_bindings_Ecase_l x P1 c e P2 :
+  unique_bindings (Ecase x (P1 ++ ((c, e) :: P2))) ->
+  unique_bindings e /\
+  unique_bindings (Ecase x P1) /\  unique_bindings (Ecase x P2) /\
+  Disjoint var (bound_var (Ecase x P1)) (bound_var e) /\
+  Disjoint var (bound_var (Ecase x P2)) (bound_var e) /\
+  Disjoint var (bound_var (Ecase x P1)) (bound_var (Ecase x P2)).
+Proof.
+  intros H. induction P1.
+  - inv H. split; [ assumption |].
+    split; [now constructor |]. split; [assumption |].
+    split.
+    + rewrite bound_var_Ecase_nil. now apply Disjoint_Empty_set_l.
+    + split.
+      * now apply Disjoint_sym.
+      * rewrite bound_var_Ecase_nil. now apply Disjoint_Empty_set_l.
+  - inv H. destruct (IHP1 H3) as [H1' [H2' [H3' [H4' [H5' H6']]]]].
+    split; [ assumption |].
+    split.
+    + constructor; [ assumption | assumption |].
+      rewrite !bound_var_Ecase_append, !bound_var_Ecase_cons in *.
+      eapply Disjoint_sym. eapply Disjoint_Union_l.
+      eapply Disjoint_sym. eassumption.
+    + split; [ assumption |]. split.
+      * rewrite !bound_var_Ecase_append, !bound_var_Ecase_cons in *.
+        eapply Disjoint_Union; [| assumption ].
+        eapply Disjoint_Included_r; [| eassumption ].
+        eapply Included_Union_mon_r.
+        eapply Included_Union_l.
+      * split; [ assumption |].
+        rewrite !bound_var_Ecase_append, !bound_var_Ecase_cons in *.
+        eapply Disjoint_Union; [| assumption ].
+        eapply Disjoint_Included_r; [| eassumption ].
+        do 2eapply Included_Union_mon_r. apply Included_refl.
+Qed.
+
+Lemma unique_bindings_Ecase_r x P1 c e P2 :
+  unique_bindings e ->
+  unique_bindings (Ecase x P1) ->
+  unique_bindings (Ecase x P2) ->
+  Disjoint var (bound_var (Ecase x P1)) (bound_var e) ->
+  Disjoint var (bound_var (Ecase x P2)) (bound_var e) ->
+  Disjoint var (bound_var (Ecase x P1)) (bound_var (Ecase x P2)) ->
+  unique_bindings (Ecase x (P1 ++ ((c, e) :: P2))).
+Proof.
+  intros H1 H2 H3 H4 H5 H6. induction P1 as [| [c' e'] P1 IHP1].
+  - constructor; [assumption | assumption |].
+    now apply Disjoint_sym.
+  - inv H2. 
+    simpl. rewrite !bound_var_Ecase_cons in *. constructor; [| eassumption |].
+    * eapply IHP1; [ assumption | |].
+      eapply Disjoint_Union_r. eassumption.
+      eapply Disjoint_Union_r. eassumption.
+    * rewrite !bound_var_Ecase_append in *.
+      eapply Disjoint_sym.
+      eapply Disjoint_Union; [ eapply Disjoint_sym; eassumption |].
+      rewrite bound_var_Ecase_cons. 
+      eapply Disjoint_Union; eapply Disjoint_sym;
+      now eapply Disjoint_Union_l; eauto.
+Qed.
+
 (** The set of names of the functions in the same fix definition *)
 Fixpoint fundefs_names (defs : fundefs) : FVSet :=
   match defs with
@@ -597,10 +826,9 @@ Lemma bound_var_fundefs_Fcons f tau xs e B1 :
                          (Union var (bound_var e) (bound_var_fundefs B1)))).
 Proof.
   split; intros x H; inv H; eauto.
-  inv H6; eauto.
-  constructor; eauto.
-  inv H0. constructor; eauto.
-  inv H. constructor 3; eauto. constructor 2; eauto.
+  - inv H6; eauto.
+  - inv H0. now eauto.
+    inv H; now eauto.
 Qed.
 
 Lemma bound_var_fundefs_Fnil  :
@@ -608,7 +836,6 @@ Lemma bound_var_fundefs_Fnil  :
 Proof.
   split; intros x H; inv H; eauto.
 Qed.
-
 
 
 Lemma split_fds_bound_vars B1 B2 B3 :
@@ -685,31 +912,29 @@ Proof.
   - inv Hun1. constructor; eauto.
     + intros Hc. apply H5. 
       eapply (split_fds_bound_vars) in Hc; eauto. inv Hc; eauto.
-      inv HD. exfalso. eapply H0. constructor; eauto.
-      constructor; eauto.
+      inv HD. exfalso. eapply H0. now eauto.
     + rewrite split_fds_bound_vars; eauto.
       constructor. intros x H. inv H. inv H0; eauto.
-      eapply H7. constructor; eauto.
-      eapply HD; constructor; eauto. constructor; eauto.
+      eapply H7. now eauto.
+      eapply HD. now eauto.
     + rewrite split_fds_bound_vars; eauto.
       constructor. intros x H. inv H. inv H1; eauto.
-      eapply H8. constructor; eauto. 
-      eapply HD; constructor; eauto. constructor 3; eauto.
+      eapply H8. now eauto.
+      eapply HD; now eauto.
     + eapply IHHspl; eauto. rewrite bound_var_fundefs_Fcons in HD.
       repeat apply Disjoint_Union_r in HD; eauto.
   - inv Hun2. constructor; eauto.
     + intros Hc. apply H5. 
       eapply (split_fds_bound_vars) in Hc; eauto. inv Hc; eauto.
-      inv HD. exfalso. eapply H0. constructor; eauto.
-      constructor; eauto.
+      inv HD. exfalso. eapply H0. now eauto.
     + rewrite split_fds_bound_vars; eauto.
       constructor. intros x H. inv H. inv H0; eauto.
-      eapply HD; constructor; eauto. constructor; eauto.
-      eapply H7. constructor; eauto.
+      eapply HD; now eauto.
+      eapply H7. now eauto.
     + rewrite split_fds_bound_vars; eauto.
       constructor. intros x H. inv H. inv H1; eauto.
-      eapply HD; constructor; eauto. constructor 3; eauto.
-      eapply H8. constructor; eauto. 
+      eapply HD; now eauto.
+      eapply H8. now eauto.
     + eapply IHHspl; eauto. rewrite bound_var_fundefs_Fcons in HD.
       apply Disjoint_sym in HD. repeat apply Disjoint_Union_r in HD; eauto.
       apply Disjoint_sym; eauto.
@@ -929,12 +1154,14 @@ Proof.
                (big_cup (fun_in_fundefs B2) _)).
   rewrite <- Union_big_cup.
   eapply Same_Set_big_cup_l. rewrite split_fds_fun_in_fundefs; eauto.
-  apply Same_set_refl.
-  eapply Same_set_Union_compat; eapply Same_Set_big_cup_r;
-  intros [[[f tau] xs] e]; rewrite Setminus_Union; rewrite <- Union_assoc.
-  rewrite split_fds_name_in_fundefs; eauto. apply Same_set_refl.
+  now apply Same_set_refl.
+  eapply Same_set_Union_compat; eapply Same_Set_big_cup_r.
+  intros [[[f tau] xs] e]. rewrite !Setminus_Union.
+  rewrite split_fds_name_in_fundefs; eauto. now apply Same_set_refl.
+  intros [[[f tau] xs] e]. rewrite !Setminus_Union.
+  rewrite split_fds_name_in_fundefs; eauto.
   rewrite (Union_sym (name_in_fundefs B2) (name_in_fundefs B1)).
-  rewrite split_fds_name_in_fundefs; eauto. apply Same_set_refl.
+  now apply Same_set_refl.
 Qed.
 
 Lemma split_fds_closed_fundefs B1 B2 B3 :
@@ -955,7 +1182,6 @@ Lemma bound_var_Efun B e :
            (Union var (bound_var_fundefs B) (bound_var e)).
 Proof.
   split; intros x H; inv H; eauto.
-  apply Bound_Efun1; eauto. apply Bound_Efun2; eauto.
 Qed.
   
 Lemma unique_bindings_hoist B1 B2 B3 f tau xs e B B' :
@@ -968,20 +1194,18 @@ Proof.
   intros Hsp1 Hsp2 Hsp3 Hun.
   edestruct split_fds_unique_bindings_fundefs_l as [H1 [H2 H3]]; eauto.
   assert (Hun2 : unique_bindings_fundefs B2).
-  { eapply split_fds_unique_bindings_fundefs_r; [ | | | apply Hsp2 ]; eauto.
-    inv H2. rewrite bound_var_Efun in *. constructor; eauto. intros H. apply H7.
-    apply Bound_Efun2; eauto.
-    eapply Disjoint_Union_r; eauto.
-    eapply Disjoint_Union_r; eauto.
-    inv H13; eauto.
-    rewrite bound_var_fundefs_Fcons in *.
-    eapply Disjoint_Included_r; eauto.
-    repeat apply Included_Union_compat; eauto using Included_refl.
-    rewrite bound_var_Efun. apply Included_Union_r. }
+  { eapply split_fds_unique_bindings_fundefs_r; [ | | | now apply Hsp2 ]; eauto.
+    - inv H2. rewrite bound_var_Efun in *. constructor; eauto.
+      now eapply Disjoint_Union_r; eauto.
+      now eapply Disjoint_Union_r; eauto.
+      now inv H13; eauto.
+    - rewrite bound_var_fundefs_Fcons in *.
+      eapply Disjoint_Included_r; eauto.
+      repeat apply Included_Union_compat; eauto using Included_refl.
+      rewrite bound_var_Efun. apply Included_Union_r. }
   edestruct split_fds_unique_bindings_fundefs_l as [H1' [H2' H3']]; eauto.
   eapply split_fds_unique_bindings_fundefs_r; [ | | | eauto]; eauto.
-  inv H2. inv H13; eauto.
-  inv H2.
+  inv H2. inv H13; eauto. inv H2.
   rewrite (split_fds_bound_vars B1 (Fcons f tau xs e Fnil) B2); eauto.
   rewrite bound_var_fundefs_Fcons in *. rewrite bound_var_Efun in *.
   apply Disjoint_sym. apply Disjoint_Union.
@@ -1087,8 +1311,7 @@ Proof.
       eapply find_def_not_name_in_fundefs. intros Hc.
       symmetry in Heq. apply fundefs_append_split_fds in Heq.
       edestruct split_fds_unique_bindings_fundefs_l as [H1 [H2 H3]]; eauto.
-      eapply H3. constructor; eauto. apply name_in_fundefs_bound_var_fundefs; eauto.
-      rewrite bound_var_fundefs_Fcons. left; eauto.
+      eapply H3. constructor; eauto. apply name_in_fundefs_bound_var_fundefs; now eauto.
     + edestruct split_fds_cons_l_append_fundefs as [B1' [B2' [Heq Hspl3]]]; eauto.
       erewrite Heq. rewrite find_def_fundefs_append_Fcons_neq; eauto.
       inv Hun. apply IHHspl1; eauto.
@@ -1103,7 +1326,6 @@ Proof.
       symmetry in Heq. apply fundefs_append_split_fds in Heq.
       edestruct split_fds_unique_bindings_fundefs_l as [H1 [H2 H3]]; eauto.
       eapply H3. constructor; eauto. apply name_in_fundefs_bound_var_fundefs; eauto.
-      rewrite bound_var_fundefs_Fcons. left; eauto.
     + edestruct split_fds_cons_r_append_fundefs as [B1' [B2' [Heq Hspl3]]]; eauto.
       erewrite Heq. rewrite find_def_fundefs_append_Fcons_neq; eauto.
       inv Hun. apply IHHspl1; eauto.
@@ -1169,6 +1391,186 @@ Proof.
     intros y Hin Hc. eapply Hall; eauto. right; eauto.
 Qed.
 
+Open Scope ctx_scope.
+
+Lemma bound_var_comp_mut :
+  (forall c e e', Same_set _ (bound_var e) (bound_var e') ->
+                  Same_set _ (bound_var (c |[ e ]|)) (bound_var (c |[ e' ]|))) /\
+  (forall B e e', Same_set _ (bound_var e) (bound_var e') ->
+                  Same_set _ (bound_var_fundefs (B <[ e ]>))
+                           (bound_var_fundefs (B <[ e' ]>))).
+Proof.
+  exp_fundefs_ctx_induction IHc IHf; eauto; simpl.
+  - intros e1 e2 H.
+    rewrite !bound_var_Econstr, IHc; [| eassumption ].
+    apply Same_set_refl.
+  - intros e1 e2 H.
+    rewrite !bound_var_Eproj, IHc; [| eassumption ].
+    apply Same_set_refl.
+  - intros e1 e2 H.
+    rewrite !bound_var_Eprim, IHc; [| eassumption ].
+    apply Same_set_refl.
+  - intros l' e1 e2 H.
+    rewrite !bound_var_Ecase_append, !bound_var_Ecase_cons, IHc; [| eassumption ].
+    apply Same_set_refl.
+  - intros e1 e2 H.
+    rewrite !bound_var_Efun, IHc; [| eassumption ].
+    apply Same_set_refl.
+  - intros e1 e2 H.
+    rewrite !bound_var_Efun, IHf; [| eassumption ].
+    apply Same_set_refl.
+  - intros e1 e2 H.
+    rewrite !bound_var_fundefs_Fcons, IHc; [| eassumption ].
+    apply Same_set_refl.
+  - intros e1 e2 H.
+    rewrite !bound_var_fundefs_Fcons, IHf; [| eassumption ].
+    apply Same_set_refl.
+Qed. 
+
+Corollary bound_var_comp c e e' :
+  Same_set _ (bound_var e) (bound_var e') ->
+  Same_set _ (bound_var (c |[ e ]|)) (bound_var (c |[ e' ]|)).
+Proof.
+  apply bound_var_comp_mut.
+Qed.
+
+Corollary bound_var_fundefs_comp B e e' :
+   Same_set _ (bound_var e) (bound_var e') ->
+   Same_set _ (bound_var_fundefs (B <[ e ]>))
+            (bound_var_fundefs (B <[ e' ]>)).
+Proof.
+  apply bound_var_comp_mut.
+Qed.
+
+
+Lemma unique_bindings_ctx_mut :
+  (forall c e e', unique_bindings (c |[ e ]|) -> unique_bindings e' ->
+                  Same_set _ (bound_var e) (bound_var e') ->
+                  unique_bindings (c |[ e' ]|)) /\
+  (forall B e e', unique_bindings_fundefs (B <[ e ]>) -> unique_bindings e' ->
+                  Same_set _ (bound_var e) (bound_var e') ->
+                  unique_bindings_fundefs (B <[ e' ]>)).
+Proof.
+  exp_fundefs_ctx_induction IHc IHf; eauto; simpl; eauto;
+  try (intros e1 e2 Hun Hun' HS;
+       inv Hun; constructor; [| now eauto ];
+       intros Hc; apply H1;
+       eapply bound_var_comp; eassumption).
+  - intros l' e1 e2 Hun Hun' HS.
+    edestruct unique_bindings_Ecase_l as [H1' [H2' [H3' [H4' [H5' H6']]]]].
+    eassumption.
+    eapply unique_bindings_Ecase_r; try eassumption.
+    + eapply IHc; eassumption.
+    + rewrite bound_var_comp. eassumption.
+      now apply Same_set_sym.
+    + rewrite bound_var_comp. eassumption.
+      now apply Same_set_sym.
+  - intros e1 e2 Hun Hun' HS.
+    inv Hun. constructor; [| eassumption |].
+    eapply IHc; eassumption.
+    rewrite bound_var_comp. eassumption.
+    now apply Same_set_sym.
+  - intros e1 e2 Hun Hun' HS.
+    inv Hun. constructor; [eassumption | |].
+    eapply IHf; eassumption.
+    rewrite bound_var_fundefs_comp. eassumption.
+    now apply Same_set_sym.
+  - intros e1 e2 Hun Hun' HS.
+    inv Hun. constructor; try eassumption.
+    + intros Hc. apply H4.
+      eapply bound_var_comp; eassumption.
+    + rewrite bound_var_comp. eassumption.
+      now apply Same_set_sym.
+    + rewrite bound_var_comp. eassumption.
+      now apply Same_set_sym.
+    + eapply IHc; eassumption.
+  - intros e1 e2 Hun Hun' HS.
+    inv Hun. constructor; try eassumption.
+    + intros Hc. apply H5.
+      eapply bound_var_fundefs_comp; eassumption.
+    + rewrite bound_var_fundefs_comp. eassumption.
+      now apply Same_set_sym.
+    + rewrite bound_var_fundefs_comp. eassumption.
+      now apply Same_set_sym.
+    + eapply IHf; eassumption.
+Qed.
+
+Lemma unique_bindings_ctx c e e':
+  unique_bindings (c |[ e ]|) -> unique_bindings e' ->
+  Same_set _ (bound_var e) (bound_var e') ->
+  unique_bindings (c |[ e' ]|).
+Proof.
+  eapply unique_bindings_ctx_mut.
+Qed.
+
+Lemma unique_bindings_fundefs_ctx B e e':
+  unique_bindings_fundefs (B <[ e ]>) -> unique_bindings e' ->
+  Same_set _ (bound_var e) (bound_var e') ->
+  unique_bindings_fundefs (B <[ e' ]>).
+Proof.
+  eapply unique_bindings_ctx_mut.
+Qed.
+
+Lemma name_in_fundefs_ctx B e1 e2 :
+  Same_set _ (name_in_fundefs (B <[ e1 ]>)) (name_in_fundefs (B <[ e2 ]>)).
+Proof.
+  induction B; simpl; (apply Same_set_Union_compat; [ now apply Same_set_refl |]).
+  now apply Same_set_refl.
+  eassumption.
+Qed.
+
+Lemma occurs_free_comp_mut :
+  (forall c e e', Same_set _ (occurs_free e) (occurs_free e') ->
+                  Same_set _ (occurs_free (c |[ e ]|)) (occurs_free (c |[ e' ]|))) /\
+  (forall B e e', Same_set _ (occurs_free e) (occurs_free e') ->
+                  Same_set _ (occurs_free_fundefs (B <[ e ]>)) (occurs_free_fundefs (B <[ e' ]>))).
+Proof.
+  exp_fundefs_ctx_induction IHc IHf; eauto; simpl.
+  - intros e1 e2 H. rewrite !occurs_free_Econstr, IHc; [| eassumption ].
+    apply Same_set_refl.
+  - intros e1 e2 H. rewrite !occurs_free_Eproj, IHc; [| eassumption ].
+    apply Same_set_refl.
+  - intros e1 e2 H. rewrite !occurs_free_Eprim, IHc; [| eassumption ].
+    apply Same_set_refl.
+  - intros l' e1 e2 H. rewrite !occurs_free_Ecase_app, IHc; [| eassumption ].
+    apply Same_set_refl.
+  - intros e1 e2 H. rewrite !occurs_free_Efun, IHc; [| eassumption ].
+    apply Same_set_refl.
+  - intros e1 e2 H. rewrite !occurs_free_Efun, IHf; [| eassumption ].
+    rewrite name_in_fundefs_ctx. apply Same_set_refl.
+  - intros e1 e2 H. rewrite !occurs_free_fundefs_Fcons, IHc; [| eassumption ].
+    apply Same_set_refl.
+  - intros e1 e2 H. rewrite !occurs_free_fundefs_Fcons, IHf; [| eassumption ].
+    rewrite name_in_fundefs_ctx. apply Same_set_refl.
+Qed.
+
+Corollary occurs_free_comp :
+  forall c e e', Same_set _ (occurs_free e) (occurs_free e') ->
+                 Same_set _ (occurs_free (c |[ e ]|)) (occurs_free (c |[ e' ]|)).
+Proof.
+  apply occurs_free_comp_mut.
+Qed.
+
+Corollary occurs_free_fundefs_comp :
+  forall B e e', Same_set _ (occurs_free e) (occurs_free e') ->
+                 Same_set _ (occurs_free_fundefs (B <[ e ]>)) (occurs_free_fundefs (B <[ e' ]>)).
+Proof.
+  apply occurs_free_comp_mut.
+Qed.
+
+Lemma funs_in_fundef_split_fds (B1 B2 B3 : fundefs) B :
+  split_fds B1 B2 B3 ->
+  funs_in_fundef B B3 ->
+  funs_in_fundef B B1 \/ funs_in_fundef B B2.
+Proof.
+  intros H1 H2; induction H1; eauto.
+  - inv H2.
+    + left; eauto.
+    + destruct IHsplit_fds; eauto.
+  - inv H2.
+    + right; eauto.
+    + destruct IHsplit_fds; eauto.
+Qed.
 
 (** Equivalence of computational and inductive FV definitions *)
 
